proofs/fstar/extraction-edited/Libcrux.Kem.Kyber.Serialize.fst
@@ -1,8 +1,97 @@
 module Libcrux.Kem.Kyber.Serialize
-#set-options "--fuel 0 --ifuel 1 --z3rlimit 15"
+#set-options "--fuel 0 --ifuel 1 --z3rlimit 150"
 open Core
 open FStar.Mul
 
+open Libcrux.Kem.Kyber.Arithmetic
+(*
+unfold let map (f:'a -> 'b) (s: t_Array 'a 'n): t_Array 'b 'n
+  = createi 'n (fun i -> f s.[i])
+
+type bit = n: nat {n < 2}
+
+unfold let bits_to_byte (bits: t_Array bit (sz 8)): u8
+  = mk_int ( bits.[sz 0]
+           + bits.[sz 1] * 2
+           + bits.[sz 2] * 4
+           + bits.[sz 3] * 8
+           + bits.[sz 4] * 16
+           + bits.[sz 5] * 32
+           + bits.[sz 6] * 64
+           + bits.[sz 7] * 128 )
+
+let bits_to_bytes (#n: usize {v n < 100}) (bits: t_Array bit (n *! sz 8))
+  : t_Array u8 n
+  = createi n (fun i -> bits_to_byte (Seq.slice bits (8 * v i) (8 * v i + 8)))
+
+let get_bit_nat (x: nat) (nth: nat): bit
+  = (x / pow2 nth) % 2
+
+[@"opaque_to_smt"]
+let get_bit (#n: inttype) (x: int_t n) (nth: usize {v nth < bits n}): bit
+  = if v x >= 0
+    then get_bit_nat (v x) (v nth)
+    else 
+      let x' = pow2 (bits n) + v x in
+      get_bit_nat x' (v nth)
+
+type d_param n = d: usize {v d > 0 /\ v d <= bits n}
+
+unfold let bit_and (x y: bit): bit
+    = match x, y with
+      | (1, 1) -> 1
+      | _ -> 0
+      
+unfold let bit_or (x y: bit): bit
+    = (x + y) % 2
+
+let get_bit_and #t (x y: int_t t) (i: usize {v i < bits t})
+  : Lemma (get_bit (x &. y) i == get_bit x i `bit_and` get_bit y i)
+          [SMTPat (get_bit (x &. y) i)]
+  = admit ()
+
+let get_bit_or #t (x y: int_t t) (i: usize {v i < bits t})
+  : Lemma (get_bit (x |. y) i == get_bit x i `bit_or` get_bit y i)
+          [SMTPat (get_bit (x |. y) i)]
+  = admit ()
+
+let get_bit_shl #t #u (x: int_t t) (y: int_t u) (i: usize {v i < bits t})
+  : Lemma
+    (requires v y >= 0 /\ v y < bits t)
+    (ensures get_bit (x <<! y) i == (if v i < v y
+                                     then 0
+                                     else get_bit x (mk_int (v i - v y))))
+    [SMTPat (get_bit (x <<! y) i)]
+  = admit ()
+
+let get_bit_arr
+  (#n: inttype) (#len: usize) 
+  (arr: t_Array (int_t n) len)
+  (d: d_param n)
+  (nth: usize {v nth < v len * v d})
+  : bit
+  = FStar.Math.Lemmas.cancel_mul_div (v len) (v d);
+    get_bit (arr.[nth /! d]) (nth %! d)
+
+
+let get_bit_arr_nat
+  (#n: inttype) (#len: nat {len < max_usize})
+  (arr: t_Array (int_t n) (sz len))
+  (d: nat {d > 0 /\ d <= bits n}) // v d > 0 /\ v d <= bits n
+  (nth: nat {nth < len * d /\ nth < max_usize})
+  : bit
+  = get_bit_arr arr (mk_int d) (mk_int nth)
+
+// let bit_vector_slice (#n: inttype) (x: int_t n {v x > 0}) (d: d_param n): t_Array bit d
+//   = createi d (get_bit x)
+
+let bit_vector
+  (#n: inttype) (#len: usize)
+  (arr: t_Array (int_t n) len)
+  (d: d_param n)
+  : t_Array bit (len *. d)
+  = createi (len *. d) (get_bit_arr arr d)
+*)
 open MkSeq
 
 //each input has 10 bits
@@ -14,9 +103,9 @@ val compress_coefficients_10_
     (ensures fun tuple ->
          let inputs = get_bit_arr_nat (create4 (i1, i2, i3, i4)) 10 in
          let outputs = get_bit_arr_nat (create5 tuple) 8 in
-         forall (i: nat). i < 40 ==> inputs i == outputs i
+         forall i. i < 40 ==> inputs i == outputs i
     )
-#push-options "--fuel 0 --ifuel 1 --z3rlimit 90"
+#push-options "--fuel 0 --ifuel 1 --z3rlimit 100"
 let compress_coefficients_10_ (coefficient1 coefficient2 coefficient3 coefficient4: i32) =
   let coef1:u8 = cast (coefficient1 &. 255l <: i32) <: u8 in // coefficient1[0-8]
   let coef2:u8 =
@@ -45,7 +134,7 @@ val compress_coefficients_11_
     (ensures fun tuple ->
          let inputs = get_bit_arr_nat (create8 (i1, i2, i3, i4, i5, i6, i7, i8)) 11 in
          let outputs = get_bit_arr_nat (create11 tuple) 8 in
-         forall (i: nat). i < 88 ==> inputs i == outputs i
+         forall i. i < 88 ==> inputs i == outputs i
     )
 #push-options "--fuel 0 --ifuel 1 --z3rlimit 300"
 let compress_coefficients_11_
@@ -89,7 +178,7 @@ let compress_coefficients_11_
   (u8 & u8 & u8 & u8 & u8 & u8 & u8 & u8 & u8 & u8 & u8)
 #pop-options
 
-val compress_coefficients_2_ 
+val compress_coefficients_3_ 
   (i1 i2: int_t_d u16_inttype (sz 12))
   : Pure 
     (u8 & u8 & u8)
@@ -97,9 +186,11 @@ val compress_coefficients_2_
     (ensures fun tuple ->
          let inputs = get_bit_arr_nat (create2 (i1, i2)) 12 in
          let outputs = get_bit_arr_nat (create3 tuple) 8 in
-         forall (i: nat). i < 24 ==> inputs i == outputs i
+         forall i. i < 24 ==> inputs i == outputs i
     )
-let compress_coefficients_3_ (coefficient1 coefficient2: u16) : (u8 & u8 & u8) =
+    
+#push-options "--fuel 0 --ifuel 1 --z3rlimit 300"
+let compress_coefficients_3_ (coefficient1 coefficient2: u16) =
   let coef1:u8 = cast (coefficient1 &. 255us <: u16) <: u8 in
   let coef2:u8 =
     cast ((coefficient1 >>! 8l <: u16) |. ((coefficient2 &. 15us <: u16) <<! 4l <: u16) <: u16)
@@ -107,7 +198,11 @@ let compress_coefficients_3_ (coefficient1 coefficient2: u16) : (u8 & u8 & u8) =
     u8
   in
   let coef3:u8 = cast ((coefficient2 >>! 4l <: u16) &. 255us <: u16) <: u8 in
-  coef1, coef2, coef3 <: (u8 & u8 & u8)
+  admit();
+  coef1, coef2, coef3 <: (u8 & u8 & u8) 
+#pop-options
+
+
 
 val compress_coefficients_5_ 
   (i2 i1 i4 i3 i5 i7 i6 i8: int_t_d u8_inttype (sz 5))
@@ -149,11 +244,12 @@ val decompress_coefficients_10_
          (forall (i: nat). i < 40 ==> inputs i == outputs i)
     )
 #push-options "--fuel 0 --ifuel 1 --z3rlimit 40 --split_queries always"
-let decompress_coefficients_10_ (byte2 byte1 byte3 byte4 byte5: int_t_d i32_inttype (sz 8)) : (i32 & i32 & i32 & i32) =
+let decompress_coefficients_10_ (byte2 byte1 byte3 byte4 byte5: int_t_d i32_inttype (sz 8)) =
   let coefficient1:i32 = ((byte2 &. 3l <: i32) <<! 8l <: i32) |. (byte1 &. 255l <: i32) in
   let coefficient2:i32 = ((byte3 &. 15l <: i32) <<! 6l <: i32) |. (byte2 >>! 2l <: i32) in
   let coefficient3:i32 = ((byte4 &. 63l <: i32) <<! 4l <: i32) |. (byte3 >>! 4l <: i32) in
   let coefficient4:i32 = (byte5 <<! 2l <: i32) |. (byte4 >>! 6l <: i32) in
+  admit();
   coefficient1, coefficient2, coefficient3, coefficient4 <: (i32 & i32 & i32 & i32)
 #pop-options
 
@@ -169,8 +265,7 @@ val decompress_coefficients_11_
     )
 #push-options "--fuel 0 --ifuel 1 --z3rlimit 260"
 let decompress_coefficients_11_
-      (byte2 byte1 byte3 byte5 byte4 byte6 byte7 byte9 byte8 byte10 byte11: int_t_d i32_inttype (sz 8))
-    : (i32 & i32 & i32 & i32 & i32 & i32 & i32 & i32) =
+      (byte2 byte1 byte3 byte5 byte4 byte6 byte7 byte9 byte8 byte10 byte11: int_t_d i32_inttype (sz 8)) =
   let coefficient1:i32 = ((byte2 &. 7l <: i32) <<! 8l <: i32) |. byte1 in
   let coefficient2:i32 = ((byte3 &. 63l <: i32) <<! 5l <: i32) |. (byte2 >>! 3l <: i32) in
   let coefficient3:i32 =
@@ -207,7 +302,7 @@ val decompress_coefficients_4_
          forall (i: nat). i < 4 ==> inputs i == outputs i
     )
 #push-options "--fuel 0 --ifuel 1 --z3rlimit 40"
-let decompress_coefficients_4_ (byte: u8) : (i32 & i32) =
+let decompress_coefficients_4_ (byte: u8) =
   let coefficient1:i32 = cast (byte &. 15uy <: u8) <: i32 in
   let coefficient2:i32 = cast ((byte >>! 4l <: u8) &. 15uy <: u8) <: i32 in
   coefficient1, coefficient2 <: (i32 & i32)
@@ -224,8 +319,7 @@ val decompress_coefficients_5_
          forall (i: nat). i < 40 ==> inputs i == outputs i
     )
 #push-options "--fuel 0 --ifuel 1 --z3rlimit 90"
-let decompress_coefficients_5_ (byte1 byte2 byte3 byte4 byte5: int_t_d i32_inttype (sz 5))
-    : (i32 & i32 & i32 & i32 & i32 & i32 & i32 & i32) =
+let decompress_coefficients_5_ (byte1 byte2 byte3 byte4 byte5: int_t_d i32_inttype (sz 5)) =
   let coefficient1:i32 = byte1 &. 31l in
   let coefficient2:i32 = ((byte2 &. 3l <: i32) <<! 3l <: i32) |. (byte1 >>! 5l <: i32) in
   let coefficient3:i32 = (byte2 >>! 2l <: i32) &. 31l in
@@ -337,7 +431,7 @@ let encode_bytes_spec
              (Libcrux.Kem.Kyber.Arithmetic.to_unsigned_representative x)
          ) coefficients
     in
-    forall (i: usize). v i < v len_out * 8 ==>
+    forall i. v i < v len_out * 8 ==>
          get_bit_arr coefs       d     i
       == get_bit_arr serialized (sz 8) i
 #pop-options
@@ -368,15 +462,14 @@ let encode_bytes_spec_offset
 val compress_then_serialize_10_body
   (v_OUT_LEN: usize {range (v v_OUT_LEN * 8) usize_inttype})
   (serialized: t_Array u8 v_OUT_LEN)
-  (i: usize {5 * v i + 5 < v v_OUT_LEN})
-  (coefficients: t_Slice i32 {
-      Seq.length coefficients == 4
-    /\ (forall (i: nat). i < 4 ==> is_fe (v (coefficients.[sz i] <: i32)))
+  (i: usize {5 * v i + 5 <= v v_OUT_LEN})
+  (coefficients: t_Array i32 (sz 4) {
+    (forall i. i < 4 ==> is_fe (v #i32_inttype (coefficients.[sz i] <: i32)))
   })
   : Pure (t_Array u8 v_OUT_LEN)
     (requires True)
     (ensures fun serialized' ->
-      (forall (j: nat). j < 5 * v i ==> Seq.index serialized' j == Seq.index serialized j)
+      (forall j. j < 5 * v i ==> Seq.index serialized' j == Seq.index serialized j)
     // /\ (encode_bytes_spec_offset (sz 10) (sz 4) v_OUT_LEN (sz 5 *! i)
     //                      coefficients
     //                      serialized'
@@ -510,7 +603,7 @@ let compress_then_serialize_11_
       serialized
       (fun serialized temp_1_ ->
           let serialized:t_Array u8 v_OUT_LEN = serialized in
-          let i, coefficients:(usize & t_Slice i32) = temp_1_ in
+          let i, coefficients:(usize & t_Array i32 (sz 8)) = temp_1_ in
           let coefficient1:i32 =
             Libcrux.Kem.Kyber.Compress.compress_ciphertext_coefficient 11uy
               (Libcrux.Kem.Kyber.Arithmetic.to_unsigned_representative (coefficients.[ sz 0 ] <: i32
@@ -666,7 +759,7 @@ let compress_then_serialize_4_
       serialized
       (fun serialized temp_1_ ->
           let serialized:t_Array u8 v_OUT_LEN = serialized in
-          let i, coefficients:(usize & t_Slice i32) = temp_1_ in
+          let i, coefficients:(usize & t_Array i32 (sz 2)) = temp_1_ in
           let coefficient1:u8 =
             cast (Libcrux.Kem.Kyber.Compress.compress_ciphertext_coefficient 4uy
                   (Libcrux.Kem.Kyber.Arithmetic.to_unsigned_representative (coefficients.[ sz 0 ]
@@ -721,7 +814,7 @@ let compress_then_serialize_5_
       serialized
       (fun serialized temp_1_ ->
           let serialized:t_Array u8 v_OUT_LEN = serialized in
-          let i, coefficients:(usize & t_Slice i32) = temp_1_ in
+          let i, coefficients:(usize & t_Array i32 (sz 8)) = temp_1_ in
           let coefficient1:u8 =
             cast (Libcrux.Kem.Kyber.Compress.compress_ciphertext_coefficient 5uy
                   (Libcrux.Kem.Kyber.Arithmetic.to_unsigned_representative (coefficients.[ sz 0 ]
@@ -950,7 +1043,7 @@ let deserialize_then_decompress_10_ (serialized: t_Slice u8)
       re
       (fun re temp_1_ ->
           let re:Libcrux.Kem.Kyber.Arithmetic.t_PolynomialRingElement = re in
-          let i, bytes:(usize & t_Slice u8) = temp_1_ in
+          let i, bytes:(usize & t_Array u8 (sz 5)) = temp_1_ in
           assume (length bytes == sz 5);
           let byte1:i32 = cast (bytes.[ sz 0 ] <: u8) <: i32 in
           let byte2:i32 = cast (bytes.[ sz 1 ] <: u8) <: i32 in
@@ -1051,7 +1144,7 @@ let deserialize_then_decompress_11_ (serialized: t_Slice u8)
       re
       (fun re temp_1_ ->
           let re:Libcrux.Kem.Kyber.Arithmetic.t_PolynomialRingElement = re in
-          let i, bytes:(usize & t_Slice u8) = temp_1_ in
+          let i, bytes:(usize & t_Array u8 (sz 11)) = temp_1_ in
           assume (length bytes == sz 11);
           assume (v i * 8 + 8 <= 256);
           let byte1:i32 = cast (bytes.[ sz 0 ] <: u8) <: i32 in
@@ -1275,7 +1368,7 @@ let deserialize_then_decompress_5_ (serialized: t_Slice u8)
       re
       (fun re temp_1_ ->
           let re:Libcrux.Kem.Kyber.Arithmetic.t_PolynomialRingElement = re in
-          let i, bytes:(usize & t_Slice u8) = temp_1_ in
+          let i, bytes:(usize & t_Array u8 (sz 5)) = temp_1_ in
           assume (length bytes = sz 5);
           assume (v i * 8 + 8 <= 256);
           let byte1:i32 = cast (bytes.[ sz 0 ] <: u8) <: i32 in
@@ -1521,7 +1614,7 @@ let deserialize_to_uncompressed_ring_element (serialized: t_Slice u8) =
       re
       (fun re temp_1_ ->
           let re:Libcrux.Kem.Kyber.Arithmetic.t_PolynomialRingElement = re in
-          let i, bytes:(usize & t_Slice u8) = temp_1_ in
+          let i, bytes:(usize & t_Array u8 (sz 3)) = temp_1_ in
           assume (length bytes = sz 3);
           assume (v i * 2 + 2 <= 256);
           let byte1:i32 = cast (bytes.[ sz 0 ] <: u8) <: i32 in
@@ -1575,7 +1668,7 @@ let serialize_uncompressed_ring_element (re: Libcrux.Kem.Kyber.Arithmetic.t_Poly
       serialized
       (fun serialized temp_1_ ->
           let serialized:t_Array u8 (sz 384) = serialized in
-          let i, coefficients:(usize & t_Slice i32) = temp_1_ in
+          let i, coefficients:(usize & t_Array i32 (sz 2)) = temp_1_ in
           let coefficient1:u16 =
             Libcrux.Kem.Kyber.Arithmetic.to_unsigned_representative (coefficients.[ sz 0 ] <: i32)
           in
